Computability/Constructions/Eval_Aux.lean
@@ -1,0 +1,103 @@
+import Computability.Constructions.Option
+
+open Nat
+open Denumerable
+open Encodable
+open List
+
+
+section rfindOpt
+namespace Nat.RecursiveIn.Code
+
+theorem rfind'_eqv_rfind : ((Nat.unpaired fun a m => (Nat.rfind fun n => (fun m => m = 0) <$> eval O c (Nat.pair a (n + m))).map (· + m)) (Nat.pair x 0)) = (Nat.rfind fun n => (fun m => m = 0) <$> eval O c (Nat.pair x n)) := by
+-- theorem rfind'_eqv_rfind : ((Nat.unpaired fun a m => (Nat.rfind fun n => (fun m => m = 0) <$> eval O c (Nat.pair a (n + m))).map (· + m)) ∘ (Nat.pair <$> (fun (n:ℕ)=>n) <*> Part.some 0)) x = (Nat.rfind fun n => (fun m => m = 0) <$> eval O c (Nat.pair x n)) := by
+  simp only [Nat.unpaired]
+  simp only [Nat.unpair_pair, add_zero, Part.map_eq_map]
+  exact rfl
+
+/--`[code_rfind c](x)=smallest n s.t. [c](x,n)=0.`-/
+-- def c_rfind : ℕ→ℕ := fun c => comp (rfind' c) (pair Nat.RecursiveIn.Code.id zero)
+def c_rfind : Nat.RecursiveIn.Code→Nat.RecursiveIn.Code := fun c => (rfind' c).comp (pair c_id zero)
+
+/-- Given a code `c` -/
+abbrev rfind (O:ℕ→ℕ) : ℕ→ℕ→.ℕ := fun c => fun a=> Nat.rfind fun n => (fun m => m = 0) <$> eval O c (Nat.pair a n)
+theorem c_rfind_prop : eval O (c_rfind c) a = (rfind O c a) := by
+  unfold c_rfind
+  unfold rfind
+  rw [←rfind'_eqv_rfind]
+  simp [eval,Seq.seq,pure,PFun.pure]
+
+theorem c_rfind_prop2 : eval O (c_rfind c) a = (Nat.rfind (fun x => n2b' <$> eval O c (Nat.pair a x))) := by
+  simp [c_rfind_prop]
+  simp [rfind]
+  unfold n2b'
+  simp
+
+def c_ppred := c_rfind (c_if_eq'.comp₂ left (succ.comp right))
+@[simp] theorem c_ppred_ev : eval O c_ppred y = Nat.ppred y := by
+  unfold c_ppred
+  simp [c_rfind_prop2]
+  simp [eval]
+  simp [Seq.seq]
+  cases y with
+  | zero =>
+    simp
+    have : ¬ ((Nat.rfind fun x ↦ Part.some (n2b' 1))).Dom := by
+      simp
+      simp [n2b']
+
+
+    exact Part.eq_none_iff'.mpr this
+  | succ n =>
+    simp
+    unfold n2b'
+    simp
+    aesop
+
+
+def c_ofOption (c:Code) := c_ppred.comp c
+theorem c_ofOption_ev (hc1:code_total O c) : eval O (c_ofOption c) x = ↑(n2o ((eval O c x).get (hc1 x))) := by
+  unfold c_ofOption
+  simp [eval]
+  simp [Part.Dom.bind (hc1 x)]
+  cases (eval O c x).get (hc1 x) with
+  | zero => simp; exact rfl
+  | succ n => simp; exact rfl
+
+-- def c_rfindOpt (c:Code) := (c_ofOption c).comp (c_rfind (c_isSome.comp (c.comp right)))
+def c_rfindOpt (c:Code) := (c_ofOption c).comp₂ c_id (c_rfind (c_isSome.comp (c)))
+@[simp] theorem c_rfindOpt_ev (hc1:code_total O c) : eval O (c_rfindOpt c) x =  Nat.rfindOpt (fun y => n2o $ (eval O c (Nat.pair x y)).get (hc1 (Nat.pair x y))) := by
+  unfold c_rfindOpt
+  simp [eval]
+  simp [c_rfind_prop2]
+  unfold rfindOpt
+  simp
+  simp [eval]
+  simp [n2b']
+  simp [b'2n]
+
+  have : ((fun x_1 ↦ (eval O c (Nat.pair x x_1)).bind fun y ↦ Part.some !decide (n2o y = Option.none))) = ((fun n ↦ Part.some (n2o ((eval O c (Nat.pair x n)).get (hc1 (Nat.pair x n)))).isSome)) := by
+
+    funext n
+    simp [Part.Dom.bind (hc1 (Nat.pair x n))]
+    cases n2o ((eval O c (Nat.pair x n)).get (hc1 (Nat.pair x n))) with
+    | none => simp
+    | some val => simp
+
+  rw [this]
+  if hh: (Nat.rfind fun n ↦ Part.some (n2o ((eval O c (Nat.pair x n)).get (hc1 (Nat.pair x n)))).isSome).Dom then
+  simp [Part.Dom.bind hh]
+  simp [Seq.seq]
+  simp [c_ofOption_ev hc1]
+  simp [Part.Dom.bind hh]
+  -- have : ((eval O c ((Nat.rfind fun n ↦ Part.some (n2o ((eval O c (Nat.pair x n)).get (hc1 (Nat.pair x n)))).isSome).get hh))).Dom := by exact hc1 ((Nat.rfind fun n ↦ Part.some (n2o ((eval O c (Nat.pair x n)).get (hc1 (Nat.pair x n)))).isSome).get hh)
+  -- congr
+  
+  
+  else
+  simp [Part.eq_none_iff'.mpr hh]
+  simp [Seq.seq]
+end Nat.RecursiveIn.Code
+-- -- theorem Nat.PrimrecIn.rfindOpt:Nat.PrimrecIn O Nat.rfindOpt := by ...
+-- -- theorem Nat.Primrec.rfindOpt:Nat.Primrec Nat.rfindOpt := by ...
+end rfindOpt
