Computability/Constructions/Option.lean
@@ -1,0 +1,31 @@
+import Computability.Constructions.Primitive
+
+open Nat
+open Denumerable
+open Encodable
+open List
+
+
+
+-- theorem option_isSome : Primrec (@Option.isSome α) :=
+--   (option_casesOn .id (const false) (const true).to₂).of_eq fun o => by cases o <;> rfl
+
+
+
+section isSome
+namespace Nat.RecursiveIn.Code
+def c_isSome := c_sg'
+@[simp] theorem c_isSome_ev_pr:code_prim c_isSome := by unfold c_isSome; repeat (first|assumption|simp|constructor)
+@[simp] theorem c_isSome_evp:eval_prim O c_isSome = fun o => b'2n $ (n2o o).isSome := by
+  simp [c_isSome]
+  funext x
+  simp
+  simp [b'2n, n2o]
+  cases x with
+  | zero => simp; exact rfl
+  | succ n => simp; exact Option.isSome_iff_ne_none.mp rfl
+@[simp] theorem c_isSome_ev:eval O c_isSome = fun o => b'2n $ (n2o o).isSome := by rw [← eval_prim_eq_eval c_isSome_ev_pr]; simp only [c_isSome_evp];
+end Nat.RecursiveIn.Code
+-- theorem Nat.PrimrecIn.isSome:Nat.PrimrecIn O Nat.isSome := by ...
+-- theorem Nat.Primrec.isSome:Nat.Primrec Nat.isSome := by ...
+end isSome
